theories/logic/olt.v
@@ -1,0 +1,126 @@
+From stdpp Require Import base.
+
+(* This file equips the type [option A] with a strict ordering [olt],
+   which is intentionally NOT well-founded: [None < None] holds. *)
+
+Section S.
+
+(* Suppose we have a type [A] equipped with a strict order [R]. *)
+
+Context `{StrictOrder A R}.
+
+(* Then, the type [option A] can be equipped with a strict ordering where
+   [None < None] holds. This ordering is NOT well-founded: indeed, [None]
+   is not accessible. [Some x] is accessible if and only if [x] is
+   accessible in the ordering of the type [A]. *)
+
+(* The type [option A], equipped with this ordering, can be used to keep
+   track of an invariant. If an element [x] does not satisfy the invariant
+   then its measure should be [None]. In other words, if [x] is accessible
+   then [x] satisfies the invariant. Thus, a witness of accessibility is,
+   at the same time, a witness that the invariant is satisfied. *)
+
+Implicit Type o : option A.
+
+Definition olt o1 o2 :=
+  match o1, o2 with
+  | None, None =>
+      True (* loop! *)
+  | None, Some _
+  | Some _, None =>
+      False
+  | Some x1, Some x2 =>
+      R x1 x2
+  end.
+
+(* We define the non-strict ordering [ole] as the union of [olt] and
+   equality. Other definitions come to mind, but this one suits our
+   purposes. *)
+
+Definition ole o1 o2 :=
+  olt o1 o2 ∨ o1 = o2.
+
+(* Local notations, lemmas, and tactics. *)
+
+Declare Scope option_scope.
+Local Infix "<" := olt (at level 70) : option_scope.
+Local Infix "≤" := ole (at level 70) : option_scope.
+Local Open Scope option_scope.
+
+Local Lemma R_trans x y z : R x y → R y z → R x z.
+Proof. intros. transitivity y; eauto. Qed.
+
+Local Ltac injections :=
+  repeat match goal with h: Some ?o1 = Some ?o2 |- _ =>
+    injection h; clear h; intro
+  end; try subst.
+
+(* Properties of [olt]. *)
+
+Lemma olt_refl o : o = None → o < o.
+Proof. intro. subst. simpl. tauto. Qed.
+
+Lemma olt_trans o0 o1 o2 : o0 < o1 → o1 < o2 → o0 < o2.
+Proof.
+  destruct o0 as [o0|]; destruct o1 as [o1|]; destruct o2 as [o2|];
+  unfold olt; eauto using R_trans.
+  + tauto.
+Qed.
+
+(* Properties of [ole]. *)
+
+Lemma ole_refl o : o ≤ o.
+Proof. unfold ole. eauto. Qed.
+
+Lemma ole_trans o0 o1 o2 : o0 ≤ o1 → o1 ≤ o2 → o0 ≤ o2.
+Proof.
+  unfold ole. intros [|] [|]; subst; eauto using olt_trans.
+Qed.
+
+Lemma ole_olt_trans o0 o1 o2 : o0 ≤ o1 → o1 < o2 → o0 < o2.
+Proof.
+  unfold ole. intros [|] ?; subst; eauto using olt_trans.
+Qed.
+
+Lemma olt_ole_trans o0 o1 o2 : o0 < o1 → o1 ≤ o2 → o0 < o2.
+Proof.
+  unfold ole. intros ? [|]; subst; eauto using olt_trans.
+Qed.
+
+Lemma olt_ole o0 o1 : o0 < o1 → o0 ≤ o1.
+Proof. unfold ole. eauto. Qed.
+
+(* [Some x] at type [option A] is accessible if and only if
+   [x] at type [A] is accessible. *)
+
+Lemma Acc_Some : ∀ x, Acc R x → Acc olt (Some x).
+Proof.
+  induction 1. constructor. intros x' ?.
+  (* [x'] cannot be [None]. *)
+  destruct x' as [x'|]; simpl in *; [ eauto | tauto ].
+Qed.
+
+(* If [A] is well-founded then every [Some x] is accessible. *)
+
+Lemma wf_Some : well_founded R → ∀ x, Acc olt (Some x).
+Proof.
+  unfold well_founded. eauto using Acc_Some.
+Qed.
+
+(* [None] is not accessible. *)
+
+Local Lemma Acc_None_aux : ∀ x, Acc olt x → x = None → False.
+Proof.
+  induction 1. intro. subst x.
+  clear H0. rename H1 into IH.
+  eapply IH; [| reflexivity ].
+  (* [None < None] is true. *)
+  reflexivity.
+Qed.
+
+Lemma Acc_None : ¬ Acc olt None.
+Proof.
+  unfold not. eauto using Acc_None_aux.
+Qed.
+
+End S.
